theories/InductionTest.v
@@ -1,8 +1,0 @@
-From Stdlib Require Import Arith.
-
-Type lt_wf_double_rect.
-Print lt_wf_double_rect.
-
-Goal forall a b, a + b = 0.
-intros.
-induction a, b using lt_wf_double_rect.
